Foundation/Modal/Boxdot/Grz_S.lean
@@ -4,8 +4,6 @@ import Foundation.Modal.Boxdot.GL_S
 namespace LO.Modal.Logic
 
 lemma iff_provable_Grz_provable_boxdot_S : Modal.S ⊢! φᵇ ↔ Modal.Grz ⊢! φ := by
-  apply Iff.trans iff_provable_boxdot_GL_provable_boxdot_S.symm;
-  simp only [Hilbert.Normal.iff_logic_provable_provable];
-  exact iff_provable_boxdot_GL_provable_Grz;
+  apply Iff.trans iff_provable_boxdot_GL_provable_boxdot_S.symm iff_provable_boxdot_GL_provable_Grz;
 
 end LO.Modal.Logic
