Foundation/Modal/Boxdot/K4_S4.lean
@@ -8,10 +8,10 @@ namespace LO.Modal
 open LO.Entailment LO.Entailment.FiniteContext LO.Modal.Entailment
 open Formula
 
-lemma provable_boxdotTranslated_K4_of_provable_S4 : Modal.S4 ⊢! φ → Hilbert.K4 ⊢! φᵇ :=
-  Hilbert.of_provable_boxdotTranslated_axiomInstances $ by
+lemma provable_boxdotTranslated_K4_of_provable_S4 : Modal.S4 ⊢! φ → Modal.K4 ⊢! φᵇ :=
+  Hilbert.Normal.of_provable_boxdotTranslated_axiomInstances $ by
     intro φ hp;
-    rcases (by simpa using hp) with (⟨_, _, rfl⟩ | ⟨_, rfl⟩ | ⟨_, rfl⟩);
+    rcases (by simpa [Axiom.instances] using hp) with (⟨_, _, rfl⟩ | ⟨_, rfl⟩ | ⟨_, rfl⟩);
     . exact boxdot_axiomK!;
     . exact boxdot_axiomT!;
     . exact boxdot_axiomFour!
@@ -22,10 +22,10 @@ lemma provable_S4_iff_boxdotTranslated : Modal.S4 ⊢! φ ⭤ φᵇ := by
   | himp φ ψ ihp ihq => exact ECC!_of_E!_of_E! ihp ihq;
   | _ => exact E!_id;
 
-lemma provable_S4_of_provable_boxdotTranslated_K4 (h : Hilbert.K4 ⊢! φᵇ) : Modal.S4 ⊢! φ := by
+lemma provable_S4_of_provable_boxdotTranslated_K4 (h : Modal.K4 ⊢! φᵇ) : Modal.S4 ⊢! φ := by
   exact (K!_right provable_S4_iff_boxdotTranslated) ⨀ (WeakerThan.pbl h);
 
-theorem iff_boxdotTranslatedK4_S4 : Hilbert.K4 ⊢! φᵇ ↔ Modal.S4 ⊢! φ := ⟨
+theorem iff_boxdotTranslatedK4_S4 : Modal.K4 ⊢! φᵇ ↔ Modal.S4 ⊢! φ := ⟨
   provable_S4_of_provable_boxdotTranslated_K4,
   provable_boxdotTranslated_K4_of_provable_S4
 ⟩
