Foundation/Modal/Maximal/Makinson.lean
@@ -24,7 +24,6 @@ open LO.Entailment LO.Entailment.FiniteContext LO.Modal.Entailment
 
 lemma KD_subset_of_not_subset_Ver.lemma₁ (hL : L ⊢! φ) (hV : Modal.Ver ⊬ φ) : ∃ ψ, L ⊢! ◇ψ := by
   obtain ⟨ψ, ⟨Γ, rfl⟩, h⟩ := Hilbert.NNFormula.exists_CNF φ;
-  replace h := Modal.Hilbert.Normal.iff_logic_provable_provable.mpr h;
   generalize eγ : (⋀Γ.unattach).toFormula = γ at h;
 
   have : L ⊢! φ.toNNFormula.toFormula ⭤ γ := WeakerThan.pbl h;
@@ -46,8 +45,7 @@ lemma KD_subset_of_not_subset_Ver.lemma₁ (hL : L ⊢! φ) (hV : Modal.Ver ⊬ 
 lemma KD_subset_of_not_subset_Ver (hV : ¬L ⪯ Modal.Ver) : Modal.KD ⪯ L := by
   apply weakerThan_iff.mpr;
   intro φ hφ;
-  simp only [Hilbert.Normal.iff_logic_provable_provable] at hφ;
-  replace hφ : Hilbert.KP ⊢! φ := Entailment.Equiv.iff.mp inferInstance _ |>.mpr hφ;
+  replace hφ : Modal.KP ⊢! φ := Entailment.Equiv.iff.mp inferInstance _ |>.mpr hφ;
   induction hφ using Hilbert.Normal.rec! with
   | axm _ h =>
     rcases h with (rfl | rfl);
@@ -109,7 +107,6 @@ lemma KD_provability_of_classical_satisfiability (hl : φ.Letterless) :
       tauto;
     . intro h;
       have : Modal.KD ⊢! □(∼φ) := nec! $ ihφ (by grind) |>.2 $ by tauto;
-      simp only [Hilbert.Normal.iff_logic_provable_provable] at ⊢ this;
       exact negbox_dne'! $ dia_duality'!.mp $ axiomD'! this;
 
 lemma provable_KD_of_classical_satisfiability (hl : φ.Letterless) : (v ⊧ φᵀ.toPropFormula) → Modal.KD ⊢! φ :=
@@ -157,9 +154,7 @@ lemma subset_Triv_of_KD_subset.lemma₂ {φ : Modal.Formula α} {s : Proposition
 theorem subset_Triv_of_KD_subset [Modal.KD ⪯ L] : L ⪯ Modal.Triv := by
   by_contra! hC;
   obtain ⟨φ, hφ₁, hφ₂⟩ := not_weakerThan_iff.mp hC;
-  replace hφ₂ := (not_imp_not.mpr Propositional.Hilbert.Cl.completeness)
-    $ Modal.Logic.Triv.iff_provable_Cl.not.mp
-    $ Hilbert.Normal.iff_logic_provable_provable.not.mp hφ₂
+  replace hφ₂ := (not_imp_not.mpr Propositional.Hilbert.Cl.completeness) $ Modal.Triv.iff_provable_Cl.not.mp $ hφ₂;
   obtain ⟨s, h⟩ := ClassicalSemantics.exists_neg_zeroSubst_of_not_isTautology hφ₂;
   let ψ := φ⟦(s : Modal.ZeroSubstitution _).1⟧;
   have : Semantics.Valid (ClassicalSemantics.Valuation ℕ) (∼(ψᵀ.toPropFormula)) := subset_Triv_of_KD_subset.lemma₂.mp h;
@@ -181,13 +176,13 @@ theorem makinson : (L.VerFamily ∨ L.TrivFamily) ∧ ¬(L.VerFamily ∧ L.TrivF
     . have := KD_subset_of_not_VerFamily h;
       exact subset_Triv_of_KD_subset (L := L);
   . by_contra hC;
+    apply Logic.no_bot (L := Modal.Ver);
     have ⟨⟨hVer⟩, ⟨hKD, hTriv⟩⟩ := hC;
     have : Modal.KD ⪯ Modal.Ver := by apply Entailment.WeakerThan.trans (𝓣 := L) <;> infer_instance;
     have h₁ : Modal.Ver ⊢! ∼□⊥ := by apply Entailment.WeakerThan.pbl (show Modal.KD ⊢! ∼□⊥ by simp);
     have h₂ : Modal.Ver ⊢! □⊥ := by simp;
     have : Modal.Ver ⊢! ⊥ := h₁ ⨀ h₂;
-    apply Entailment.Consistent.not_bot inferInstance (𝓢 := Modal.Ver);
-    simpa;
+    assumption;
 
 lemma VerFamily.notTrivFamily [L.VerFamily] : ¬L.TrivFamily := by
   apply not_and.mp $ makinson (L := L) |>.2;
