Foundation/Modal/ModalCompanion/Cl.lean
@@ -3,7 +3,7 @@ import Foundation.Modal.Kripke.Logic.S5Grz
 import Foundation.Modal.Boxdot.Ver_Triv
 import Foundation.Propositional.Kripke.Logic.Cl
 
-namespace LO
+namespace LO.Modal
 
 open LO.Entailment LO.Entailment.FiniteContext LO.Modal.Entailment
 open Propositional
@@ -13,150 +13,121 @@ open Modal
 open Modal.Kripke
 open Modal.Formula.Kripke
 
-namespace Propositional
 
-lemma Logic.Cl.smallestMC.mem_diabox_box : (smallestMC 𝐂𝐥) ⊢! (◇□(.atom 0) ➝ □(.atom 0)) := by
-  have : (smallestMC 𝐂𝐥) ⊢! □(.atom 0) ⋎ □(∼□(.atom 0)) := by
+lemma smallestMC_of_Cl.mem_diabox_box : (𝐂𝐥.smallestMC) ⊢! (◇□(.atom 0) ➝ □(.atom 0)) := by
+  have H₁ : (𝐂𝐥.smallestMC) ⊢! □(.atom 0) ⋎ □(∼□(.atom 0)) := by
     apply Logic.sumNormal.mem₂!;
     use Axioms.LEM (.atom 0);
     constructor;
     . simp [theory];
     . tauto;
-  apply _ ⨀ this;
-  apply C!_trans ?_ CANC!;
-  apply C!_trans ?_ or_comm!;
-  apply CAA!_of_C!_of_C!;
-  . simp;
-  . apply CN!_of_CN!_right;
-    exact diaDuality_mp!;
+  have H₂ : 𝐂𝐥.smallestMC ⊢! ◇□(.atom 0) ➝ ∼□(∼□(.atom 0)) := diaDuality_mp!;
+  cl_prover [H₁, H₂];
 
-instance : Entailment.HasAxiomFive (smallestMC 𝐂𝐥) where
+instance : Entailment.HasAxiomFive (𝐂𝐥.smallestMC) where
   Five φ := by
     constructor;
     apply Modal.Logic.iff_provable.mp;
-    apply Modal.Logic.subst! (L := (smallestMC 𝐂𝐥)) (φ := Modal.Axioms.Five (.atom 0)) (s := λ a => φ);
-    have := Modal.Logic.subst! (s := λ _ => ∼(.atom 0)) $ Logic.Cl.smallestMC.mem_diabox_box;
-    apply _ ⨀ this;
-    apply C!_trans ?_ CANC!;
-    apply C!_trans CCAN! ?_;
-    apply C!_trans ?_ or_comm!;
-    apply CAA!_of_C!_of_C!;
-    . apply CN!_of_CN!_left;
-      exact diaDuality_mp!;
-    . apply CN!_of_CN!_right;
-      exact diaDuality_mp!;
+    apply Modal.Logic.subst! (L := (𝐂𝐥.smallestMC)) (φ := Modal.Axioms.Five (.atom 0)) (s := λ a => φ);
+    have H₁ : 𝐂𝐥.smallestMC ⊢! ◇□(∼.atom 0) ➝ □(∼.atom 0) := Modal.Logic.subst! (s := λ _ => ∼(.atom 0)) $ smallestMC_of_Cl.mem_diabox_box;
+    have H₂ : 𝐂𝐥.smallestMC ⊢! ∼□◇(.atom 0) ➝ ◇□(∼.atom 0) := diaDuality_mp!;
+    have H₃ : 𝐂𝐥.smallestMC ⊢! ◇(.atom 0) ➝ ∼□(∼.atom 0) := diaDuality_mp!;
+    cl_prover [H₁, H₂, H₃];
 
-end Propositional
+namespace S5
 
-
-namespace Modal
-
-open LO.Entailment LO.Entailment.FiniteContext LO.Modal.Entailment
-open Propositional
-open Propositional.Formula (goedelTranslate)
-open Propositional.Formula (atom)
-open Modal
-open Modal.Kripke
-
-section S5
-
-namespace Logic
-
-lemma S5.is_smallestMC_of_Cl : Modal.S5 = (smallestMC 𝐂𝐥) := by
-  apply Logic.iff_equal_provable_equiv.mpr;
-  apply Entailment.Equiv.antisymm_iff.mpr;
+instance : Modal.S5 ≊ 𝐂𝐥.smallestMC := by
+  apply Logic.equiv_of_provable;
+  intro φ;
   constructor;
-  . apply Entailment.weakerThan_iff.mpr;
-    intro φ hφ;
-    simp only [Hilbert.Normal.iff_logic_provable_provable] at hφ;
+  . intro hφ;
     induction hφ using Modal.Hilbert.Normal.rec! with
-    | axm _ h => rcases h with (rfl | rfl | rfl) <;> simp;
+    | axm s h =>
+      rcases h with (rfl | rfl | rfl | rfl) <;> simp;
     | mdp ihφψ ihφ => exact ihφψ ⨀ ihφ;
     | nec ihφ => exact nec! ihφ;
     | _ => simp;
-  . apply Entailment.weakerThan_iff.mpr;
-    intro _ hφ;
+  . intro hφ;
     induction hφ using Logic.sumNormal.rec! with
     | mem₁ h => apply WeakerThan.pbl h;
     | mdp ihφψ ihψ => exact ihφψ ⨀ ihψ;
     | nec ihφ => exact nec! ihφ;
-    | subst ihφ => apply subst! _ ihφ;
+    | subst ihφ => apply Logic.subst! _ ihφ;
     | mem₂ h =>
-      apply Hilbert.Normal.iff_logic_provable_provable.mpr;
       rcases h with ⟨φ, hφ, rfl⟩;
-      apply rm_diabox'!;
-      apply WeakerThan.pbl (𝓢 := Modal.S4);
-      exact (diaK'! $ goedelTranslated_axiomTc) ⨀ (iff_provable_Cl_provable_dia_gS4.mp hφ);
+      apply provable_goedelTranslated_of_provable Hilbert.Cl Modal.S5;
+      . rintro _ ⟨_, (rfl | rfl), ⟨s, rfl⟩⟩;
+        . simp;
+        . apply rm_diabox'!;
+          apply WeakerThan.pbl (𝓢 := Modal.S4);
+          apply (diaK'! $ goedelTranslated_axiomTc) ⨀ (iff_provable_Cl_provable_dia_gS4.mp _);
+          simp [theory];
+      . simpa [theory] using hφ;
 
-instance : Sound (smallestMC 𝐂𝐥) FrameClass.S5 := by
-  rw [←Logic.S5.is_smallestMC_of_Cl];
-  infer_instance;
+lemma is_smallestMC_of_Cl : Modal.S5 = 𝐂𝐥.smallestMC := Logic.eq_of_equiv
 
-instance modalCompanion_Cl_S5 : ModalCompanion 𝐂𝐥 Modal.S5 := by
-  rw [Logic.S5.is_smallestMC_of_Cl];
-  apply Modal.instModalCompanion_of_smallestMC_via_KripkeSemantics
+instance : Sound (𝐂𝐥.smallestMC) FrameClass.S5 := Kripke.sound_frameClass_of_equiv Modal.S5 𝐂𝐥.smallestMC
+
+instance : ModalCompanion 𝐂𝐥 Modal.S5 := by
+  apply is_smallestMC_of_Cl ▸ Modal.instModalCompanion_of_smallestMC_via_KripkeSemantics
+    (IL := 𝐂𝐥)
     (IC := Propositional.Kripke.FrameClass.Cl)
     (MC := Modal.Kripke.FrameClass.S5)
-  intro F hF;
+  rintro F hF;
   simp_all only [Set.mem_setOf_eq];
   constructor;
-
-end Logic
 
 end S5
 
 
+instance : 𝐂𝐥.smallestMC ⪯ Modal.S5Grz := calc
+  _ ≊ Modal.S5    := by symm; infer_instance;
+  _ ⪯ Modal.S5Grz := inferInstance
+
+
 section S5Grz
 
-lemma Logic.gS5Grz_of_Cl : 𝐂𝐥 ⊢! φ → Modal.S5Grz ⊢! φᵍ := by
-  intro h;
-  apply WeakerThan.pbl $ modalCompanion_Cl_S5.companion.mp h;
 
-lemma Logic.S5Grz.is_largestMC_of_Cl : Modal.S5Grz = (Logic.largestMC 𝐂𝐥) := by
-  apply Logic.iff_equal_provable_equiv.mpr;
-  apply Entailment.Equiv.antisymm_iff.mpr;
+instance : Modal.S5Grz ≊ 𝐂𝐥.largestMC := by
+  apply Logic.equiv_of_provable;
+  intro φ;
   constructor;
-  . apply Entailment.weakerThan_iff.mpr;
-    intro _ hφ;
-    simp only [Hilbert.Normal.iff_logic_provable_provable] at hφ;
+  . intro hφ;
     induction hφ using Modal.Hilbert.Normal.rec! with
     | axm _ h =>
       rcases h with (rfl | rfl | rfl | rfl);
       . simp;
       . simp;
-      . apply WeakerThan.pbl (𝓢 := (smallestMC 𝐂𝐥));
-        simp;
+      . apply WeakerThan.pbl (𝓢 := 𝐂𝐥.smallestMC); simp;
       . simp;
-    | mdp ihφψ ihφ => exact ihφψ ⨀ ihφ;
-    | nec ihφ => exact nec! ihφ;
-    | _ => simp;
-  . apply Entailment.weakerThan_iff.mpr;
-    intro φ hφ;
-    induction hφ using Logic.sumNormal.rec! with
-    | mem₁ h => apply WeakerThan.pbl $ Logic.S5.is_smallestMC_of_Cl ▸ h;
     | mdp ihφψ ihψ => exact ihφψ ⨀ ihψ;
-    | subst ih => apply subst! _ ih;
+    | nec ihφ => exact nec! ihφ;
+    | _ => apply Logic.sumNormal.mem₁!; simp;
+  . intro hφ;
+    induction hφ using Logic.sumNormal.rec! with
+    | mdp ihφψ ihψ => exact ihφψ ⨀ ihψ;
+    | subst ih => apply Logic.subst! _ ih;
     | nec ih => apply nec! ih;
+    | mem₁ h => apply WeakerThan.pbl h;
     | mem₂ h => rcases h with ⟨φ, hφ, rfl⟩; simp;
 
-instance : Sound (Logic.largestMC 𝐂𝐥) FrameClass.finite_Triv := by
-  rw [←Logic.S5Grz.is_largestMC_of_Cl];
-  infer_instance;
+lemma is_largestMC_of_KC : Modal.S5Grz = 𝐂𝐥.largestMC := Logic.eq_of_equiv
 
-instance modalCompanion_Cl_S5Grz : ModalCompanion 𝐂𝐥 Modal.S5Grz := by
-  rw [Logic.S5Grz.is_largestMC_of_Cl];
-  apply Modal.instModalCompanion_of_largestMC_via_KripkeSemantics
+instance : Sound 𝐂𝐥.largestMC FrameClass.finite_Triv := Kripke.sound_frameClass_of_equiv Modal.S5Grz 𝐂𝐥.largestMC
+
+end S5Grz
+
+
+instance S5Grz.modalCompanion : ModalCompanion 𝐂𝐥 Modal.S5Grz := by
+  apply is_largestMC_of_KC ▸ Modal.instModalCompanion_of_largestMC_via_KripkeSemantics
     (IC := Propositional.Kripke.FrameClass.finite_Cl)
     (MC := Modal.Kripke.FrameClass.finite_Triv);
   . intro F hF; simp_all only [Set.mem_setOf_eq]; exact {};
 
-instance modalCompanion_Cl_Triv : ModalCompanion 𝐂𝐥 Modal.Triv := by
-  convert modalCompanion_Cl_S5Grz;
-  apply Logic.iff_equal_provable_equiv.mpr;
-  apply Entailment.Equiv.symm
-  infer_instance;
-
-end S5Grz
+instance Triv.modalCompanion : ModalCompanion 𝐂𝐥 Modal.Triv := by
+  convert S5Grz.modalCompanion;
+  have : Modal.Triv ≊ Modal.S5Grz := by symm; infer_instance;
+  apply Logic.eq_of_equiv;
 
 
 section boxdot
@@ -165,5 +136,6 @@ theorem embedding_Cl_Ver {φ : Propositional.Formula ℕ} : 𝐂𝐥 ⊢! φ ↔
   Iff.trans ModalCompanion.companion Logic.iff_boxdotTranslated_Ver_Triv.symm
 
 end boxdot
+
 
 end LO.Modal
