Foundation/Modal/ModalCompanion/LC.lean
@@ -13,29 +13,12 @@ open Modal
 open Modal.Kripke
 open Modal.Formula.Kripke
 
-section S4Point3
-
-lemma S4Point3.goedelTranslated_axiomDummett : Modal.S4Point3 ⊢! □(□ψᵍ ➝ χᵍ) ➝ □(ψᵍ ➝ χᵍ) := by
-  apply axiomK'!;
-  apply nec!;
-  apply C!_swap;
-  apply deduct'!;
-  apply deduct!;
-  have h₁ : [□ψᵍ ➝ χᵍ, ψᵍ] ⊢[Modal.S4Point3]! ψᵍ ➝ □ψᵍ := of'! $ goedelTranslated_axiomTc;
-  have h₂ : [□ψᵍ ➝ χᵍ, ψᵍ] ⊢[Modal.S4Point3]! ψᵍ := by_axm!;
-  have h₃ : [□ψᵍ ➝ χᵍ, ψᵍ] ⊢[Modal.S4Point3]! □ψᵍ ➝ χᵍ := by_axm!;
-  exact h₃ ⨀ (h₁ ⨀ h₂);
-
 @[simp]
 lemma S4.CCLL_CCL : Modal.S4 ⊢! □(□φ ➝ □ψ) ➝ □(□φ ➝ ψ) := by
   apply Complete.complete (𝓜 := FrameClass.S4);
   rintro F ⟨_, _⟩ V x h₁ y Rxy h₂;
   apply @h₁ y Rxy h₂;
   apply IsRefl.refl;
-
-namespace Logic
-
-instance : Entailment.S4 Modal.S4 where
 
 instance : Entailment.HasAxiomPoint3 (smallestMC 𝐋𝐂) where
   Point3 φ ψ := by
@@ -53,96 +36,102 @@ instance : Entailment.HasAxiomPoint3 (smallestMC 𝐋𝐂) where
     . apply Entailment.WeakerThan.pbl (𝓢 := Modal.S4);
       simp;
 
-lemma S4Point3.is_smallestMC_of_LC : Modal.S4Point3 = (smallestMC 𝐋𝐂) := by
-  apply Logic.iff_equal_provable_equiv.mpr;
-  apply Entailment.Equiv.antisymm_iff.mpr;
+namespace S4Point3
+
+lemma goedelTranslated_axiomDummett : Modal.S4Point3 ⊢! □(□ψᵍ ➝ χᵍ) ➝ □(ψᵍ ➝ χᵍ) := by
+  apply axiomK'!;
+  apply nec!;
+  apply C!_swap;
+  apply deduct'!;
+  apply deduct!;
+  have h₁ : [□ψᵍ ➝ χᵍ, ψᵍ] ⊢[Modal.S4Point3]! ψᵍ ➝ □ψᵍ := of'! $ goedelTranslated_axiomTc;
+  have h₂ : [□ψᵍ ➝ χᵍ, ψᵍ] ⊢[Modal.S4Point3]! ψᵍ := by_axm!;
+  have h₃ : [□ψᵍ ➝ χᵍ, ψᵍ] ⊢[Modal.S4Point3]! □ψᵍ ➝ χᵍ := by_axm!;
+  exact h₃ ⨀ (h₁ ⨀ h₂);
+
+instance : Modal.S4Point3 ≊ 𝐋𝐂.smallestMC := by
+  apply Logic.equiv_of_provable;
+  intro φ;
   constructor;
-  . apply Entailment.weakerThan_iff.mpr;
-    intro φ hφ;
-    simp only [Hilbert.Normal.iff_logic_provable_provable] at hφ;
+  . intro hφ;
     induction hφ using Modal.Hilbert.Normal.rec! with
     | axm s h =>
       rcases h with (rfl | rfl | rfl | rfl) <;> simp;
     | mdp ihφψ ihφ => exact ihφψ ⨀ ihφ;
     | nec ihφ => exact nec! ihφ;
     | _ => simp;
-  . apply Entailment.weakerThan_iff.mpr;
-    intro _ hφ;
+  . intro hφ;
     induction hφ using Logic.sumNormal.rec! with
     | mem₁ h => apply WeakerThan.pbl h;
     | mdp ihφψ ihψ => exact ihφψ ⨀ ihψ;
     | nec ihφ => exact nec! ihφ;
-    | subst ihφ => apply subst! _ ihφ;
+    | subst ihφ => apply Logic.subst! _ ihφ;
     | mem₂ h =>
-      apply Hilbert.Normal.iff_logic_provable_provable.mpr;
       rcases h with ⟨φ, hφ, rfl⟩;
       apply provable_goedelTranslated_of_provable Hilbert.LC Modal.S4Point3;
-      . rintro _ ⟨_, ⟨(rfl | rfl), ⟨s, rfl⟩⟩⟩;
+      . rintro _ ⟨_, (rfl | rfl), ⟨s, rfl⟩⟩;
         . simp;
         . apply A!_replace axiomPoint3! <;>
           apply S4Point3.goedelTranslated_axiomDummett;
       . simpa [theory] using hφ;
 
-instance : Sound (smallestMC 𝐋𝐂) FrameClass.S4Point3 := by
-  rw [←Logic.S4Point3.is_smallestMC_of_LC];
-  infer_instance;
+lemma eq_smallestMC_of_KC : Modal.S4Point3 = 𝐋𝐂.smallestMC := Logic.eq_of_equiv
 
-instance modalCompanion_LC_S4Point3 : ModalCompanion 𝐋𝐂 Modal.S4Point3 := by
-  rw [Logic.S4Point3.is_smallestMC_of_LC];
-  apply Modal.instModalCompanion_of_smallestMC_via_KripkeSemantics
+instance : Sound 𝐋𝐂.smallestMC FrameClass.S4Point3 := Kripke.sound_frameClass_of_equiv Modal.S4Point3 𝐋𝐂.smallestMC
+
+instance : ModalCompanion 𝐋𝐂 Modal.S4Point3 := by
+  apply eq_smallestMC_of_KC ▸ Modal.instModalCompanion_of_smallestMC_via_KripkeSemantics
+    (IL := 𝐋𝐂)
     (IC := Propositional.Kripke.FrameClass.LC)
     (MC := Modal.Kripke.FrameClass.S4Point3)
-  intro F hF;
+  rintro F hF;
   simp_all only [Set.mem_setOf_eq];
   constructor;
-
-end Logic
 
 end S4Point3
 
 
+instance : 𝐋𝐂.smallestMC ⪯ Modal.GrzPoint3 := calc
+  _ ≊ Modal.S4Point3  := by symm; infer_instance;
+  _ ⪯ Modal.GrzPoint3 := inferInstance
+
+
+
 section GrzPoint3
 
-lemma Logic.gGrzPoint3_of_LC : 𝐋𝐂 ⊢! φ → Modal.GrzPoint3 ⊢! φᵍ := by
-  intro h;
-  apply WeakerThan.pbl $ modalCompanion_LC_S4Point3.companion.mp h;
-
-lemma Logic.GrzPoint3.is_largestMC_of_LC : Modal.GrzPoint3 = (Logic.largestMC 𝐋𝐂) := by
-  apply Logic.iff_equal_provable_equiv.mpr;
-  apply Entailment.Equiv.antisymm_iff.mpr;
+instance : Modal.GrzPoint3 ≊ 𝐋𝐂.largestMC := by
+  apply Logic.equiv_of_provable;
+  intro φ;
   constructor;
-  . apply Entailment.weakerThan_iff.mpr;
-    intro _ hφ;
-    simp only [Hilbert.Normal.iff_logic_provable_provable] at hφ;
+  . intro hφ;
     induction hφ using Modal.Hilbert.Normal.rec! with
-    | axm s h =>
+    | axm _ h =>
       rcases h with (rfl | rfl | rfl);
       . simp;
       . simp;
-      . apply WeakerThan.pbl (𝓢 := (smallestMC 𝐋𝐂));
-        simp;
-    | mdp ihφψ ihφ => exact ihφψ ⨀ ihφ;
-    | nec ihφ => exact nec! ihφ;
-    | _ => simp;
-  . apply Entailment.weakerThan_iff.mpr;
-    intro φ hφ;
-    induction hφ using Logic.sumNormal.rec! with
-    | mem₁ h => apply WeakerThan.pbl $ Logic.S4Point3.is_smallestMC_of_LC ▸ h;
+      . apply WeakerThan.pbl (𝓢 := 𝐋𝐂.smallestMC); simp;
     | mdp ihφψ ihψ => exact ihφψ ⨀ ihψ;
-    | subst ih => apply subst! _ ih;
+    | nec ihφ => exact nec! ihφ;
+    | _ => apply Logic.sumNormal.mem₁!; simp;
+  . intro hφ;
+    induction hφ using Logic.sumNormal.rec! with
+    | mdp ihφψ ihψ => exact ihφψ ⨀ ihψ;
+    | subst ih => apply Logic.subst! _ ih;
     | nec ih => apply nec! ih;
+    | mem₁ h => apply WeakerThan.pbl h;
     | mem₂ h => rcases h with ⟨φ, hφ, rfl⟩; simp;
 
-instance : Sound (Logic.largestMC 𝐋𝐂) { F : Frame | F.IsFiniteGrzPoint3' } := by
-  rw [←Logic.GrzPoint3.is_largestMC_of_LC];
-  infer_instance;
+lemma is_largestMC_of_KC : Modal.GrzPoint3 = 𝐋𝐂.largestMC := Logic.eq_of_equiv
 
-instance modalCompanion_LC_GrzPoint3 : ModalCompanion 𝐋𝐂 Modal.GrzPoint3 := by
-  rw [Logic.GrzPoint3.is_largestMC_of_LC];
-  exact Modal.instModalCompanion_of_largestMC_via_KripkeSemantics
-    (IC := Propositional.Kripke.FrameClass.finite_LC)
-    (MC := { F : Frame | F.IsFiniteGrzPoint3' })
-    (by intro F hF; simp_all only [Set.mem_setOf_eq]; exact {})
+instance : Sound 𝐋𝐂.largestMC FrameClass.finite_GrzPoint3 := Kripke.sound_frameClass_of_equiv Modal.GrzPoint3 𝐋𝐂.largestMC
+
+instance : ModalCompanion 𝐋𝐂 Modal.GrzPoint3 := by
+  apply is_largestMC_of_KC ▸ Modal.instModalCompanion_of_largestMC_via_KripkeSemantics
+    Propositional.Kripke.FrameClass.finite_LC
+    ({ F : Frame | F.IsFiniteGrzPoint3' })
+  rintro F hF;
+  simp_all only [Set.mem_setOf_eq];
+  exact {}
 
 end GrzPoint3
 
@@ -150,7 +139,7 @@ end GrzPoint3
 section boxdot
 
 theorem embedding_LC_GLPoint3 {φ : Propositional.Formula ℕ} : 𝐋𝐂 ⊢! φ ↔ Modal.GLPoint3 ⊢! φᵍᵇ :=
-  Iff.trans modalCompanion_LC_GrzPoint3.companion iff_boxdot_GLPoint3_GrzPoint3.symm
+  Iff.trans ModalCompanion.companion iff_boxdot_GLPoint3_GrzPoint3.symm
 
 end boxdot
 
