Foundation/Propositional/Kripke/Logic/KC.lean
@@ -7,7 +7,7 @@ import Foundation.Propositional.Kripke.Logic.KrieselPutnam
 namespace LO.Propositional
 
 open Kripke
-open Hilbert.Kripke
+open Modal.Kripke
 open Formula.Kripke
 
 
@@ -38,31 +38,31 @@ namespace Hilbert
 
 namespace KC.Kripke
 
-instance : Sound Hilbert.KC FrameClass.KC :=
+instance : Sound Modal.KC FrameClass.KC :=
   instSound_of_validates_axioms $ by
     apply FrameClass.Validates.withAxiomEFQ;
     rintro F hF _ rfl;
     replace hF := Set.mem_setOf_eq.mp hF;
     apply validate_axiomWeakLEM_of_isPiecewiseStronglyConvergent
 
-instance : Sound Hilbert.KC FrameClass.finite_KC :=
+instance : Sound Modal.KC FrameClass.finite_KC :=
   instSound_of_validates_axioms $ by
     apply FrameClass.Validates.withAxiomEFQ;
     rintro F hF _ rfl;
     replace hF := Set.mem_setOf_eq.mp hF;
     apply validate_axiomWeakLEM_of_isPiecewiseStronglyConvergent
 
-instance : Entailment.Consistent Hilbert.KC := consistent_of_sound_frameclass FrameClass.KC $ by
+instance : Entailment.Consistent Modal.KC := consistent_of_sound_frameclass FrameClass.KC $ by
   use whitepoint;
   apply Set.mem_setOf_eq.mpr;
   infer_instance;
 
-instance : Canonical Hilbert.KC FrameClass.KC := ⟨by
+instance : Canonical Modal.KC FrameClass.KC := ⟨by
   apply Set.mem_setOf_eq.mpr;
   infer_instance;
 ⟩
 
-instance : Complete Hilbert.KC FrameClass.KC := inferInstance
+instance : Complete Modal.KC FrameClass.KC := inferInstance
 
 section FFP
 
@@ -70,7 +70,7 @@ open
   finestFiltrationTransitiveClosureModel
   Relation
 
-instance : Complete (Hilbert.KC) FrameClass.finite_KC := ⟨by
+instance : Complete (Modal.KC) FrameClass.finite_KC := ⟨by
   intro φ hφ;
   apply Complete.complete (𝓜 := FrameClass.KC);
   rintro F F_con V r;
@@ -134,7 +134,7 @@ end FFP
 
 end KC.Kripke
 
-instance : Hilbert.KrieselPutnam ⪱ Hilbert.KC := by
+instance : Modal.KrieselPutnam ⪱ Modal.KC := by
   constructor;
   . apply weakerThan_of_subset_frameClass FrameClass.KrieselPutnam FrameClass.KC;
     intro F hF;
@@ -184,9 +184,9 @@ instance : Hilbert.KrieselPutnam ⪱ Hilbert.KC := by
         have := @F.ps_convergent _ 0 1 2;
         omega;
 
-instance : Hilbert.Int ⪱ Hilbert.KC := calc
-  Hilbert.Int ⪱ Hilbert.KrieselPutnam := inferInstance
-  _           ⪱ Hilbert.KC := inferInstance
+instance : Hilbert.Int ⪱ Modal.KC := calc
+  Hilbert.Int ⪱ Modal.KrieselPutnam := inferInstance
+  _           ⪱ Modal.KC := inferInstance
 
 end Hilbert
 
