Foundation/Propositional/Logic/Letterless_Int_Cl.lean
@@ -21,13 +21,13 @@ theorem iff_letterless_Int_Cl {φ : Formula ℕ} (hφ : φ.Letterless) : 𝐈�
   . apply WeakerThan.wk;
     infer_instance;
   . intro h;
-    have : Modal.Modal.S4 ⊢! ◇φᵍ := Modal.Logic.iff_provable_Cl_provable_dia_gS4.mp h;
-    have : Modal.Modal.Triv ⊢! ◇φᵍ := WeakerThan.pbl this;
-    have : Modal.Modal.Triv ⊢! φᵍ := diaT'! this;
-    have : (φᵍᵀ.toPropFormula _).isTautology := Modal.Logic.Triv.iff_isTautology.mp this;
+    have : Modal.S4 ⊢! ◇φᵍ := Modal.iff_provable_Cl_provable_dia_gS4.mp h;
+    have : Modal.Triv ⊢! ◇φᵍ := WeakerThan.pbl this;
+    have : Modal.Triv ⊢! φᵍ := diaT'! this;
+    have : (φᵍᵀ.toPropFormula _).isTautology := Modal.Triv.iff_isTautology.mp this;
     have : Modal.KD ⊢! φᵍ := Modal.Logic.provable_KD_of_classical_tautology (by grind) this;
     have : Modal.S4 ⊢! φᵍ := WeakerThan.pbl this;
-    exact Modal.modalCompanion_Int_S4.companion.mpr this;
+    exact Modal.ModalCompanion.companion.mpr this;
 
 end Logic
 
