Foundation/ProvabilityLogic/N/Soundness.lean
@@ -13,7 +13,7 @@ variable {L : FirstOrder.Language} [L.ReferenceableBy L]
          {T U : FirstOrder.Theory L} [T ⪯ U]
          {𝔅 : Provability T U}
 
-lemma N.arithmetical_soundness (h : Hilbert.N ⊢! A) {f : Realization 𝔅} : U ⊢! f A := by
+lemma N.arithmetical_soundness (h : Modal.N ⊢! A) {f : Realization 𝔅} : U ⊢! f A := by
   induction h using Hilbert.Normal.rec! with
   | axm _ hp => simp at hp;
   | nec ihp => exact D1_shift ihp;
